Non monotonic domains of private transition (#19)
Squashed commit of the following:

commit d6919ba3c0fccda8dd1d709cdc7a7d303e8c9edf
Author: June Rousseau <june.rousseau@cs.au.dk>
Date:   Mon Apr 14 15:52:54 2025 +0200

    Deleting non-perma state from std world in now allowed private transition

commit cf54d3c6276cd19104cf6ec2719cb20ebc65b2d1
Author: June Rousseau <june.rousseau@cs.au.dk>
Date:   Fri Apr 11 15:31:47 2025 +0200

    WIP allow non-permanent states to not be in the domain of private transitions

theories/sts.v
@@ -34,6 +34,12 @@ Notation STS_rels := (gmap positive ((positive → positive → Prop) * (positiv
 Class STS_STD (B : Type) :=
   { Rpub : relation B;
     Rpriv : relation B;
+    state_permanent : B -> Prop ; (* set of B that have to stay in the domain of the world *)
+    dec_state_permanent : forall b, Decision (state_permanent b);
+    state_permanent_reachable : forall b b', ¬ (state_permanent b) -> rtc (λ x y, (Rpub x y ∨ Rpriv x y)) b b' ;
+    state_permanent_inv : forall b b', state_permanent b
+                                         -> rtc (λ x y, (Rpub x y ∨ Rpriv x y)) b b'
+                                         -> state_permanent b' ;
   }.
 
 (** The CMRA for the sts collection. *)
@@ -107,7 +113,8 @@ Section definitionsS.
     ∀ i x y, fs !! i = Some x → gs !! i = Some y → rtc (Rpub) x y.
 
   Definition related_sts_std_priv (fs gs : STS_std_states A B) : Prop :=
-    dom fs ⊆ dom gs ∧
+    (forall i x, fs !! i = Some x -> state_permanent x -> is_Some (gs !! i) )
+    ∧
     ∀ i x y, fs !! i = Some x → gs !! i = Some y → rtc (λ x y, (Rpub x y ∨ Rpriv x y)) x y.
 
   Definition related_sts_pub (fs gs : STS_states) (fr gr : STS_rels) : Prop :=
@@ -342,9 +349,15 @@ Section STS.
     related_sts_std_pub fsd gsd → related_sts_std_priv fsd gsd.
   Proof.
     intros [Hf1 Hf2].
-    split;auto. intros i x y Hx Hy.
-    specialize (Hf2 i x y Hx Hy).
-    apply rtc_or_intro. auto.
+    split;auto.
+    - intros i x Hx Hperm_x.
+      rewrite -elem_of_dom.
+      apply Hf1.
+      rewrite elem_of_dom.
+      by exists x.
+    - intros i x y Hx Hy.
+      specialize (Hf2 i x y Hx Hy).
+      apply rtc_or_intro. auto.
   Qed.
 
   Lemma related_sts_pub_priv_world W W' :
@@ -423,14 +436,27 @@ Section STS.
     related_sts_std_priv fsd hsd.
   Proof.
     intros [Hf1 Hf2] [Hg1 Hg2]; split; try by etrans.
-    intros i x y Hx Hy.
-    specialize (Hf1 i);
-      revert Hf1; rewrite !elem_of_dom; intros Hf1.
-    destruct Hf1 as [x0 Hx0]; eauto.
-    specialize (Hf2 i x x0 Hx Hx0); simplify_eq.
-    specialize (Hg2 i x0 y Hx0 Hy); simplify_eq.
-    etrans;eauto.
-    apply rtc_or_intro; auto.
+    - intros i x Hx Hperm_x.
+      rewrite -elem_of_dom.
+      apply Hg1.
+      rewrite elem_of_dom.
+      eapply Hf1; done.
+    - intros i x y Hx Hy.
+      pose proof (dec_state_permanent x) as Hdec_x.
+      destruct (decide (state_permanent x)) as [Hperma_x|Hperma_x].
+      + specialize (Hf1 i x Hx Hperma_x).
+        destruct Hf1 as [x' Hx'].
+        specialize (Hf2 i x x' Hx Hx').
+        specialize (Hg2 i _ _ Hx' Hy).
+        clear -Hf2 Hg2.
+        eapply rtc_transitive; eauto.
+        eapply rtc_or_intro; eauto.
+      + destruct (gsd !! i) as [x'|] eqn:Hx'.
+        ++ specialize (Hf2 i x x' Hx Hx').
+           specialize (Hg2 i _ _ Hx' Hy).
+           eapply rtc_transitive; eauto.
+           eapply rtc_or_intro; eauto.
+        ++ apply (state_permanent_reachable x y Hperma_x).
   Qed.
 
   Lemma related_sts_pub_priv_trans fs fr gs gr hs hr :
@@ -456,14 +482,28 @@ Section STS.
     related_sts_std_priv fsd hsd.
   Proof.
     intros [Hf1 Hf2] [Hg1 Hg2]; split; try by etrans.
-    intros i x y Hx Hy.
-    specialize (Hf1 i);
-      revert Hf1; rewrite !elem_of_dom; intros Hf1.
-    destruct Hf1 as [x0 Hx0]; eauto.
-    specialize (Hf2 i x x0 Hx Hx0); simplify_eq.
-    specialize (Hg2 i x0 y Hx0 Hy); simplify_eq.
-    etrans;eauto.
-    apply rtc_or_intro; auto.
+    - intros i x Hx Hperm_x.
+      pose proof Hx as Hx_'.
+      eapply (elem_of_dom_2 fsd i x) in Hx.
+      eapply Hf1 in Hx.
+      rewrite elem_of_dom in Hx.
+      destruct Hx as [x' Hx].
+      assert (state_permanent x') as Hperm_x'.
+      { eapply state_permanent_inv; eauto.
+        specialize (Hf2 i x x' Hx_' Hx).
+        eapply rtc_or_intro; eauto.
+      }
+      eapply Hg1; eauto.
+    - intros i x y Hx Hy.
+      assert (is_Some (gsd !! i)) as [x' Hx'].
+      { rewrite -elem_of_dom.
+        apply Hf1.
+        by rewrite elem_of_dom.
+      }
+      specialize (Hf2 _ _ _ Hx Hx').
+      specialize (Hg2 _ _ _ Hx' Hy).
+      eapply rtc_transitive; eauto.
+      eapply rtc_or_intro; eauto.
   Qed.
 
   Lemma related_sts_priv_trans fs fr gs gr hs hr :
@@ -488,13 +528,26 @@ Section STS.
     related_sts_std_priv fsd hsd.
   Proof.
     intros [Hf1 Hf2] [Hg1 Hg2]; split; try by etrans.
-    intros i x y Hx Hy.
-    specialize (Hf1 i);
-      revert Hf1; rewrite !elem_of_dom; intros Hf1.
-    destruct Hf1 as [x0 Hx0]; eauto.
-    specialize (Hf2 i x x0 Hx Hx0); simplify_eq.
-    specialize (Hg2 i x0 y Hx0 Hy); simplify_eq.
-    etrans;eauto.
+    - intros i x Hx Hperm_x.
+      specialize (Hf1 i x Hx Hperm_x).
+      destruct Hf1 as [y Hy].
+      specialize (Hf2 i x y Hx Hy).
+      pose proof (state_permanent_inv x y Hperm_x Hf2) as Hperm_y.
+      by specialize (Hg1 i y Hy Hperm_y).
+    - intros i x y Hx Hy.
+      pose proof (dec_state_permanent x) as Hdec_x.
+      destruct (decide (state_permanent x)) as [Hperma_x|Hperma_x].
+      + specialize (Hf1 i x Hx Hperma_x).
+        destruct Hf1 as [x' Hx'].
+        specialize (Hf2 i x x' Hx Hx').
+        specialize (Hg2 i _ _ Hx' Hy).
+        clear -Hf2 Hg2.
+        eapply rtc_transitive; eauto.
+      + destruct (gsd !! i) as [x'|] eqn:Hx'.
+        ++ specialize (Hf2 i x x' Hx Hx').
+           specialize (Hg2 i _ _ Hx' Hy).
+           eapply rtc_transitive; eauto.
+        ++ apply (state_permanent_reachable x y Hperma_x).
   Qed.
 
   (* TODO helper for special *)
@@ -543,27 +596,33 @@ Section STS.
     - apply related_sts_pub_trans with W'.2.1 W'.2.2; auto.
   Qed.
 
+  Definition is_permanent_state W i :=
+    ∃ b, W.1 !! i = Some b ∧ state_permanent b.
+
   Lemma related_sts_priv_world_std_sta_is_Some W W' i :
-    related_sts_priv_world W W' -> is_Some ((W.1) !! i) -> is_Some ((W'.1) !! i).
+    related_sts_priv_world W W'
+    -> is_permanent_state W i
+    -> is_Some ((W.1) !! i)
+    -> is_Some ((W'.1) !! i).
   Proof.
-    intros [ [Hdom1 _ ] _] Hsome.
-    rewrite -elem_of_dom.
-    rewrite -elem_of_dom in Hsome.
-    apply elem_of_subseteq in Hdom1. auto.
+    intros [ [Hdom _ ] _] Hperm [x Hx].
+    destruct Hperm as [x' [Hx' Hperm_x'] ].
+    rewrite Hx' in Hx; simplify_eq.
+    by specialize (Hdom i x Hx' Hperm_x').
   Qed.
 
-  Lemma related_sts_priv_world_std_sta_region_type W W' i ρ :
-    related_sts_priv_world W W' ->
-    (W.1) !! i = Some ρ ->
-    ∃ ρ', (W'.1) !! i = Some ρ'.
-  Proof.
-    intros Hrelated Hρ.
-    assert (is_Some ((W'.1) !! i)) as [x Hx].
-    { apply related_sts_priv_world_std_sta_is_Some with W; eauto. }
-    destruct Hrelated as [ [Hdom1 Hrevoked ] _].
-    specialize (Hrevoked _ _ _ Hρ Hx). simplify_eq.
-    eauto.
-  Qed.
+  (* Lemma related_sts_priv_world_std_sta_region_type W W' i ρ : *)
+  (*   related_sts_priv_world W W' -> *)
+  (*   (W.1) !! i = Some ρ -> *)
+  (*   ∃ ρ', (W'.1) !! i = Some ρ'. *)
+  (* Proof. *)
+  (*   intros Hrelated Hρ. *)
+  (*   assert (is_Some ((W'.1) !! i)) as [x Hx]. *)
+  (*   { apply related_sts_priv_world_std_sta_is_Some with W; eauto. } *)
+  (*   destruct Hrelated as [ [Hdom1 Hrevoked ] _]. *)
+  (*   specialize (Hrevoked _ _ _ Hρ Hx). simplify_eq. *)
+  (*   eauto. *)
+  (* Qed. *)
 
   Lemma related_sts_pub_empty_world W : related_sts_pub_world (∅, (∅, ∅)) W.
   Proof.
@@ -580,7 +639,7 @@ Section STS.
   Proof.
     split; cbn.
     - split;auto.
-      + rewrite dom_empty_L; set_solver.
+      + intros ; set_solver.
       + intros ; set_solver.
     - split;auto.
       + rewrite dom_empty_L; set_solver.
@@ -843,9 +902,9 @@ Section STS.
     rewrite /related_sts_priv_world /=.
     split;[|apply related_sts_priv_refl].
     rewrite /related_sts_std_priv. split.
-    - rewrite dom_insert_L. set_solver.
-    -
-      (* apply (not_elem_of_dom (std_world W) a) in Hdom_sta. *)
+    - intros i x Hx _.
+      destruct (decide (a = i)); simplify_map_eq; done.
+    - (* apply (not_elem_of_dom (std_world W) a) in Hdom_sta. *)
       intros i x y Hx Hy.
       destruct (decide (a = i)).
       + subst. rewrite lookup_insert in Hy; simplify_eq.
