theories/region_invariants_revocation.v
@@ -1,6 +1,6 @@
 From iris.algebra Require Import gmap agree auth.
 From iris.proofmode Require Import tactics.
-From cap_machine Require Export stdpp_extra iris_extra region_invariants region_invariants_transitions.
+From cap_machine Require Export stdpp_extra iris_extra region_invariants region_invariants.
 Import uPred.
 
 Section heap.
@@ -695,13 +695,32 @@ Section heap.
         all: try (right with Temporary; [left;constructor|eright;[right; constructor|]; constructor]).
   Qed.
 
+  Lemma revoke_private_monotone_dom (Wstd_sta Wstd_sta' : gmap Addr region_type) :
+    (∀ (i : finz MemNum) (x : region_type), Wstd_sta !! i = Some x → x = Permanent → is_Some (Wstd_sta' !! i))
+    -> ( ∀ (i : finz MemNum) (x : region_type), (revoke_std_sta Wstd_sta) !! i = Some x → x = Permanent → is_Some ((revoke_std_sta Wstd_sta') !! i) ).
+  Proof.
+    intros Hmono a ρ Hρ ->.
+    assert (Wstd_sta !! a = Some Permanent).
+    { rewrite /revoke_std_sta lookup_fmap in Hρ.
+      destruct (Wstd_sta !! a); cbn in Hρ; last done.
+      destruct r;  congruence.
+    }
+    specialize (Hmono _ _ H eq_refl).
+    destruct Hmono.
+    rewrite /revoke_std_sta lookup_fmap H0.
+    destruct (decide (x = Temporary)); simplify_eq.
+    + by exists Revoked; cbn.
+    + exists x; cbn.
+      destruct x ; congruence.
+  Qed.
+
   Lemma revoke_monotone (W W' : WORLD) :
     related_sts_priv_world W W' → related_sts_priv_world (revoke W) (revoke W').
   Proof.
     destruct W as [ Wstd_sta [Wloc_sta Wloc_rel] ].
     destruct W' as [ Wstd_sta' [Wloc_sta' Wloc_rel'] ].
     intros [(Hdom_sta & Htransition) Hrelated_loc].
-    apply revoke_monotone_dom in Hdom_sta.
+    pose proof (revoke_private_monotone_dom _ _ Hdom_sta) as Hdom_sta'.
     split;[split;[auto|]|auto].
     intros i x' y' Hx' Hy'.
     simpl in *.
@@ -726,7 +745,10 @@ Section heap.
       rewrite /related_sts_std_priv.
       simpl in *.
       split.
-      + rewrite dom_insert_L. set_solver.
+      + intros a ρ Hρ ->.
+        destruct (decide (i = a)); simplify_map_eq; first done.
+        (* rewrite lookup_insert_ne; auto. *)
+        eapply Hdoms; eauto.
       + intros j x y Hx Hy.
         destruct (decide (i = j)).
         { subst.
